theories/Libs/PSLCompat.v
@@ -9,6 +9,14 @@ Proof.
 Qed.
 
 (* From PSL/Lists/BaseLists.v *)
+Lemma map_repeat (X Y : Type) (f : X -> Y) (n : nat) (a : X) :
+  map f (repeat a n) = repeat (f a) n.
+Proof.
+  induction n as [|n IHn].
+  - reflexivity.
+  - cbn. now rewrite IHn.
+Qed.
+
 Definition equi X (A B : list X) : Prop := incl A B /\ incl B A.
 Notation "A === B" := (equi A B) (at level 70).
 
@@ -42,6 +50,7 @@ Proof.
   induction xs in ys|-*;destruct ys;cbn;intros H. 1:easy. 1-2:now specialize (H 0).
   generalize (H 0).  intros [= ->]. erewrite IHxs. easy. intros n'. now specialize (H (S n')).
 Qed.
+
 Lemma vector_nth_error_nat X n' i (xs : Vector.t X n') :
   nth_error (Vector.to_list xs) i = match lt_dec i n' with
                                       Specif.left H => Some (Vector.nth xs (Fin.of_nat_lt H))
@@ -51,6 +60,10 @@ Proof.
   clear. induction xs in i|-*. now destruct i.
   cbn in *. destruct i;cbn. easy. rewrite IHxs. do 2 destruct lt_dec. 4:easy. now symmetry;erewrite Fin.of_nat_ext. all:exfalso;Lia.nia.
 Qed.
+
+Lemma vector_to_list_cast (X : Type) (n1 n2 : nat) (H : n1 = n2) (v : Vector.t X n1) :
+  Vector.to_list (Vector.cast v H) = Vector.to_list v.
+Proof. subst. rename n2 into n. induction v as [ | x n v IH]; cbn; f_equal; auto. Qed.
 
 (* From PSL/FiniteTypes/VectorFin.v *)
 Lemma Fin_cardinality n : | elem (finType_CS (Fin.t n)) | = n.
